Introduce efficient list fetch/update in Rec.v and use it in RecArray.v
Previously, RecArray's [get_item] and [put_item] would take an entire
sector, convert it into a Coq data structure, fetch/update a single
field, and re-encode it back into a sector (in the case of put_item).

This was by far the biggest cause of high CPU + memory usage in hstest,
especially in the case of the bitmap allocator, which would decode/encode
between a 512-byte sector and 4096 individual bit values.

This change introduces efficient variants for fetching and updating a
single element out of a list, without having to decode/re-encode the
entire sector: [Rec.word_selN] and [Rec.word_updN].

This gives us a 10x performance and memory use improvement for hstest;
it now takes 0.1 seconds for its 100 iterations and uses "just" 47MB
of memory.

In terms of proofs, the plan is to prove that these efficient
variants are equivalent to the naive (original) code that does full
decoding/re-encoding: these are the two theorems [Rec.word_selN_equiv]
and [Rec.word_updN_equiv].  Using these theorems, I was able to re-prove
RecArray.v.

Unfortunately, these two theorems themselves still have some [admit]s
left, mostly because of messy dependent types..

src/Rec.v
@@ -1,5 +1,7 @@
 Require Import Arith List String Omega. 
 Require Import Word.
+Require Import Eqdep_dec.
+Require Import Array.
 
 Import ListNotations.
 Open Scope string_scope.
@@ -296,15 +298,95 @@ Module Rec.
 
   Arguments of_word : simpl never.
   Arguments to_word : simpl never.
+
+
+  (**
+   * Efficient implementations for fetching or updating a single element from a
+   * [word (len (ArrayF ft len))], without decoding/encoding the whole word to
+   * and from the corresponding [list (data ft)].
+   *)
+
+  Definition middle (low mid high : nat) (w : word (low + (mid + high))) : word mid :=
+    split1 mid high (split2 low (mid+high) w).
+
+  Lemma word_selN_helper : forall idx l lenft, idx < l ->
+    l * lenft = idx * lenft + (lenft + (l * lenft - lenft - idx * lenft)).
+  Proof.
+    intros.
+    rewrite plus_assoc.
+    rewrite Nat.add_sub_assoc.
+    rewrite <- plus_assoc.
+    rewrite plus_comm.
+    rewrite <- Nat.add_sub_assoc by omega.
+    rewrite Nat.sub_diag; rewrite <- plus_n_O.
+    rewrite Nat.add_sub_assoc.
+    rewrite plus_comm.
+    rewrite <- Nat.add_sub_assoc by omega.
+    rewrite Nat.sub_diag; rewrite <- plus_n_O.
+    reflexivity.
+    replace (lenft) with (1 * lenft) at 1 by omega.
+    apply Nat.mul_le_mono_r; omega.
+    replace (lenft) with (1 * lenft) at 3 by omega.
+    rewrite <- Nat.mul_sub_distr_r.
+    apply Nat.mul_le_mono_r; omega.
+  Qed.
+
+  Definition word_selN {ft : type} {l : nat} (idx : nat) (w : word (len (ArrayF ft l))) : word (len ft).
+    refine (if lt_dec idx l then _ else $0).
+    refine (middle (idx * len ft) (len ft) (l * len ft - len ft - idx * len ft) _).
+    replace (idx * len ft + (len ft + (l * len ft - len ft - idx * len ft))) with (l * len ft).
+    exact w.
+    apply word_selN_helper.
+    apply l0.
+  Defined.
+
+  Theorem word_selN_equiv : forall ft l idx w def, idx < l ->
+    of_word (@word_selN ft l idx w) = selN (of_word w) idx def.
+  Proof.
+    induction l; intros; try omega.
+    unfold of_word in *; fold (@of_word ft) in *.
+    destruct idx; simpl.
+    - f_equal.
+      unfold word_selN, middle; simpl.
+      admit.  (* XXX dependent type mess.. *)
+    - rewrite <- IHl by omega; clear IHl.
+      f_equal.
+      unfold word_selN; simpl.
+      destruct (lt_dec (S idx) (S l)); try omega.
+      destruct (lt_dec idx l); try omega.
+      admit.  (* XXX dependent type mess.. *)
+  Qed.
+
+
+  Definition word_updN {ft : type} {l : nat} (idx : nat) (w : word (len (ArrayF ft l)))
+                                             (v : word (len ft)) : word (len (ArrayF ft l)).
+    refine (if lt_dec idx l then _ else $0); simpl in *.
+    replace (l * len ft) with (idx * len ft + (l * len ft - idx * len ft)) in *.
+    remember (split1 (idx * len ft) (l * len ft - idx * len ft) w) as low; clear Heqlow.
+    remember (split2 (idx * len ft) (l * len ft - idx * len ft) w) as midhi; clear Heqmidhi.
+    replace (l * len ft - idx * len ft) with (len ft + (l * len ft - idx * len ft - len ft)) in *.
+    remember (split1 (len ft) (l * len ft - idx * len ft - len ft) midhi) as mid; clear Heqmid.
+    remember (split2 (len ft) (l * len ft - idx * len ft - len ft) midhi) as hi; clear Heqhi.
+    refine (combine low _).
+    refine (combine v hi).
+
+    rewrite Nat.add_sub_assoc. rewrite plus_comm. rewrite <- Nat.add_sub_assoc by omega.
+    rewrite Nat.sub_diag. omega.
+
+    rewrite <- Nat.mul_sub_distr_r. replace (len ft) with (1 * len ft) at 1 by omega.
+    apply Nat.mul_le_mono_r; omega.
+
+    rewrite Nat.add_sub_assoc. rewrite plus_comm. rewrite <- Nat.add_sub_assoc by omega.
+    rewrite Nat.sub_diag. omega.
+
+    apply Nat.mul_le_mono_r; omega.
+  Defined.
+
+  Theorem word_updN_equiv : forall ft l idx w v, idx < l ->
+    @word_updN ft l idx w (to_word v) = @to_word (ArrayF ft l) (updN (of_word w) idx v).
+  Admitted.
+
 End Rec.
 
 Notation "r :-> n" := (Rec.recget' n r) (at level 20).
 Notation "r :=> n := v" := (Rec.recset' n r v) (at level 80).
-
-(*
-Definition inodetype : Rec.rectype := [("free", Rec.WordF 1); ("len", Rec.WordF 16); ("block0", Rec.WordF 16)].
-Definition inode1 : Rec.recdata inodetype := ($1, ($11, ($1677, tt))).
-Parameter inode2 : Rec.recdata inodetype.
-Definition foo := Eval compute in inode2 :-> "len".
-Definition foo2 := Eval compute in inode2 :=> "len" := $17.
-*)
